- Example #1 (20/03/2024):
	- $n=0$, $2^n=1$, $3n=0$
	- $n=1$, $2^n=2$, $3n=3$
	- $n=2$, $2^n=4$, $3n=6$
	- $n=3$, $2^n=8$, $3n=9$
	- $n=4$, $2^n=16$, $3n=12$
	- $n=5$, $2^n=32$, $3n=15$
	- $n=6$, $2^n=64$, $3n=18$
	- As $n$ goes up by one, $3n$ goes up by $3$ and $2^n$ goes up by $2^n$
	- for $n \geq 2$, $2^n$ is bigger than $3$. So if $n \geq 2$, then once $2^n > 3n$, $2^n$ stays bigger than $3n$ as $n$ gets bigger.
	- at $n=4$, $2^4 = 16 > 12 = 3 \cdot 4$
	- Claim: For any integer $n \geq 4$, $2^n > 3n$
	- Induction Goal: $2^{k+1} > 3(k+1) = 3k+3$
	- Pf:
		- (Base Case: $n=4$)
			- $2^4 = 15$
			- $3(4) = 12$
		- So $2^4 > 3(4)$
		- (Induction Case)
			- Assume that $2^k > 3k$ for some $k \in \mathbb{Z}$ where $k \geq 4$
				- $2^{k+1} = 2^k \cdot 2$
				- $> 2 \cdot 3k$
				- $= 3k + 3k$ (because $2^k > 3k$)
				- $>3k+3$ ($3k>3$ because $k \geq 4$)
				- $= 3(k+1)$
			- So $2^{k+1} > 3(k+1)$
	- **Bad Base Case:**
		- $2^4 > 3 \cdot 4$
		- $16 > 12$
	- **Okay but Weird Base Case**
		- $16 > 12$
		- $2^4 > 3$
- Example #2 (20/03/2024):
	- Claim: For any finite set $A$, if $|A| = n$, then $A$ has $2^n$ subsets $|\mathcal{P}(A)| = 2^{|A|}$
	- Goal: Every set with $k+1$ members has $2^{k+1}$ subsets
	- Pf:
	- Choose a finite set $A$, and let $n = |A|$
		- (Base Case: $n = 0$)
			- $A = \varnothing$
			- $A$ has $1$ subset, $\varnothing \subseteq \varnothing$
			- $2^0 = 1$
			- So $A$ has $2^0$ subsets
		- (Induction Case: $A$ has $k+1$ members)
			- Assume that every set with $k$ members has $2^k$ subsets for some $k \in \mathbb{N}$
				- $|A| = k+1$
				- $A = \{a_1,a_2,...,a_k,a_{k+1}\}$
				- Consider the set $A' = \{a_1,a_2,...,a_k\}$
				- $A'$ has $k$ members
				- So, by our induction hypothesis, we know $A'$ has $2^k$ subsets
				- Every subset of $A'$ is also a subset of $A$
				- If we take each subset of $A'$ and add $a_{k+1}$ to it, we get another set of $A$
			- This totals to $2^k + 2^k$ subset of $A
			- $2^k + 2^k = 2 \cdot 2^k = 2^{k+1}$
- Example #1 (25/03/2024):
	- Claim: For any $n \in \mathbb{N}$ where $n > 0$, the sum of all integers from $1$ up to $n$ is $\frac{n(n+1)}{2}$
	- Goal: $\frac{(k+1)(k+1+1)}{2}$
	- Pf:
		- (Base Case, $n=1$):
			- The sum of all integers from $1$ up to $1$ is $1$
			- $\frac{1(1+1)}{2} = \frac{2}{2} = 1$
			- So, the sum of all integer from $1$ up to $1$ is $\frac{1(1+1)}{2}$
		- (Inductive Case)
			- Assume the sum of all integers from $1$ up to $k$ is $\frac{k(k+1)}{2}$, for some int $k > 0$
			- The sum of all ints from $1$ to $k+1$ = (the sum of all ints from $1$ to $k$) + ($k+1$)
			- $= \frac{k(k+1)}{2} + (k+1)$ (because Induction Hypothesis)
			- $= \frac{k(k+1) + 2(k+1)}{2}$
			- $= \frac{(k+1)(k+2)}{2}$
			- $= \frac{(k+1)(k+1+1)}{2}$
- Example #2 (25/03/2024):
	- Claim: For any $n \in \mathbb{N}$ where $n > 0$, the sum of all integers from $1$ up to $n$ is $\frac{n(n+1)}{2}$
		- $\sum\limits^{n}_{i=1}{i}$
	- Goal: $\frac{(k+1)(k+1+1)}{2}$
	- Pf:
		- (Base Case, $n=1$):
			- The sum of all integers from $1$ up to $1$ is $1$
			- $\frac{1(1+1)}{2} = \frac{2}{2} = 1$
			- $\sum\limits^{1}_{i=1}{i} = 1$
			- So, the sum of all integer from $1$ up to $1$ is $\frac{1(1+1)}{2}$
		- (Inductive Case)
			- Assume the sum of all integers from $1$ up to $k$ is $\sum\limits^{k}_{i=1}{i}$, for some int $k > 0$
			- $\sum\limits^{k+1}_{i=1}{i} = \sum\limits^{k}_{i=1}{i} + (k+1)$
			- 
- Example #3 (25/03/2024): Summation Notation
	- $1+3+5+7+9+11$
	- $\sum\limits^{i=5}_{i=0}{2i+1}$
	- $= (2(0)+1) + (2(1)+1) + (2(2)+1) + (2(3)+1) + (2(4)+1) + (2(5)+1)$
	- $=1+3+5+6+9+11$
	- $=25$
- Example #4 (25/03/2024): Summation Notation
	- $\prod\limits^{5}_{i=1}{\frac{1}{i}} = \frac{1}{1} \cdot \frac{1}{2} \cdot \frac{1}{3} \cdot \frac{1}{4} \cdot \frac{1}{5}$
- Example #5 (25/03/2024):
	- For any $n \in \mathbb{N}$
	- Claim: $\sum\limits^{n}_{i=0}{\frac{1}{2^i}} = 2- \frac{1}{2^n}$
	- Goal: $\sum\limits^{k+1}_{i=0}{\frac{1}{2^i}} = 2- \frac{1}{2^k+1}$
	- Pf:
		- (Base Case, $n=0$)
			- $\sum\limits^{n}_{i=0}{\frac{1}{2^0}} = \sum\limits^{n}_{i=0}{\frac{1}{1}}$
			- $= \sum\limits^{n}_{i=0}{1}$
			- $= 1$
			- $=2-1$
			- $= 2-\frac{1}{1}$
			- $= 2- \frac{1}{2^0}$
		- (Inductive Case)
			- Assume $\sum\limits^{k}_{i=0}{\frac{1}{2^i}} = 2- \frac{1}{2^k}$ for some $k \in \mathbb{N}$
			- $\sum\limits^{k+1}_{i=0}{\frac{1}{2^i}} = \sum\limits^{k}_{i=0}{\frac{1}{2^i}} + \frac{1}{2^{k+1}}$
			- $= 2-\frac{1}{2^k} + \frac{1}{2^{k+1}}$ (By the Induction Hypothesis)
			- $= 2- 2(\frac{1}{2^k}) + \frac{1}{2^{k+1}}$
			- $= 2 + \frac{-1 \cdot 2}{2^k \cdot 2} + \frac{1}{2^k \cdot 2}$
			- $= 2 + \frac{-2+1}{2^k \cdot 2}$
			- $= 2 + \frac{-1}{2^k \cdot 2}$
			- $= 2 + \frac{-1}{2^k+1}$
			- $= 2 - \frac{1}{2^k+1}$
- Example #1 (17/04/2024):
	- Claim: $F_n = \frac{\varphi^n - \psi^n}{\varphi - \psi}$
	- Pf:
		- (Base, $n = 0$):
			- $\frac{\varphi^0 - \psi^0}{\varphi - \psi} = \frac{1-1}{\varphi - \psi} = 0$
			- $F_0 = 0$
		- (Base, $n=1$):
			- $\frac{\varphi^1 - \psi^1}{\varphi - \psi} = \frac{\varphi - \psi}{\varphi - \psi} = 1$
		- (Inductive Case):
			- Assume for some $k \in \mathbb{N}$, with $F_i = \frac{\varphi^i - \psi^i}{\varphi - \psi}$ for all $i \leq k$
			- $F_{k+1} = F_k + F_{k-1}$
			- $= \frac{\varphi^{k} - \psi{k}}{\varphi - \psi} + \frac{\varphi^{k-1} - \psi^{k-1}}{\varphi - \psi}$ (By IH $k \leq k$ and $k-1 \leq k$)
			- $= \frac{\varphi^k + \varphi^{k-1} - (\psi^k + \psi^{k-1})}{\varphi - \psi}$
			- $= \frac{\varphi^{k-1}(\varphi +1) - \psi^{k-1}(\psi + 1)}{\varphi - \psi}$
			- $= \frac{\varphi^{k-1}(\varphi^2) - \psi^{k-1}(\psi^2)}{\varphi - \psi}$ (As per Lemma)
			- $= \frac{\varphi^{k+1} - \psi^{k+1}}{\varphi - \psi}$
- Example #2 (17/04/2024)
	-  Claim: For any integer $n>1$, $n$ can be written as a product of prime numbers
	- Pf:
		- (Base, $n = 2$):
			- When $n=2$, we can write $2 = 2$ (a product of prime number, $n$ is)
		- (Inductive Step)
			- Assume for some integer $k > 1$, $i$ can be written as a product of prime numbers for all $i \leq k$ and $i > 1$
			- If $k+1$ is prime then, it can be written as a product of just one prime, $k+1$
			- If $k+1$ is not prime, then it can be written as $k+1 = ab$, where $a$ and $b$ are natural numbers, $2 \leq a,b \leq k$ and
				- $a,b \leq k$, so the IH says we can write both as a product of primes
				- So we can write $k+1$ as the product of these two product of primes
				- $a=p_1 \cdot p_2 \cdot p_3 \cdot \dots p_s$
				- $b=q_1 \cdot q_2 \cdot q_3 \cdot \dots q_s$